more, though slow

src/index.ts
@@ -32,6 +32,7 @@ export const range = (
   //@ verify
   //@ requires a.length > 0
   //@ requires b.length > 0
+  //@ requires forall(p: nat, p + a.length <= str.length && p + b.length <= str.length ==> (str.slice(p, p + a.length) !== a || str.slice(p, p + b.length) !== b))
   //@ ensures \result !== undefined ==> \result.length === 2
   //@ ensures \result !== undefined ==> \result[0] >= 0 && \result[0] + a.length <= str.length
   //@ ensures \result !== undefined ==> \result[1] >= 0 && \result[1] + b.length <= str.length
